theories/Iris/cointro_patterns.v
@@ -1,0 +1,100 @@
+From stdpp Require Export strings.
+From iris.proofmode Require Import base tokens.
+From iris.prelude Require Import options.
+
+Inductive goal_kind := GSpatial | GModal | GIntuitionistic.
+
+Record cointro_goal := SpecGoal {
+  cointro_goal_kind : goal_kind;
+  cointro_goal_negate : bool;
+  cointro_goal_hyps : list ident
+}.
+
+Inductive cointro_pat :=
+  | SDrop : cointro_pat 
+  | SFrame : ident → list cointro_pat → cointro_pat
+  | SFrameByName : ident → list cointro_pat → cointro_pat
+  | SPureGoal (perform_done : bool) : cointro_pat
+  | SCoHyp : ident -> cointro_pat
+  | SSplitGoal : cointro_goal → cointro_pat
+  | SRefl : cointro_pat
+  | SList : list (cointro_pat) -> cointro_pat
+.
+
+(* Definition goal_kind_modal (k : goal_kind) : bool := *)
+(*   match k with GModal => true | _ => false end. *)
+(* Definition cointro_pat_modal (p : cointro_pat) : bool := *)
+(*   match p with *)
+(*   | SSplitGoal g => goal_kind_modal (cointro_goal_kind g) *)
+(*   | _ => false *)
+(*   end. *)
+
+Module cointro_pat.
+Inductive stack_item :=
+  | StPat : cointro_pat → stack_item
+  | StFrame : string → stack_item
+  | StList : stack_item.
+Notation stack := (list stack_item).
+
+Fixpoint close (k : stack) (ps : list cointro_pat) : option (list cointro_pat) :=
+  match k with
+  | [] => Some ps
+  | StPat p :: k => close k (p :: ps)
+  | StFrame _ :: _ => None
+  | StList :: _ => None
+  end.
+
+Fixpoint close_ident (k : stack) (ps : list cointro_pat) : option stack :=
+  match k with
+  | [] => None
+  | StPat p :: k => close_ident k (p :: ps)
+  | StFrame s :: k => Some (StPat (SFrame s ps) :: k)
+  | StList :: k => Some (StPat (SList ps) :: k)
+  end.
+
+Fixpoint parse_go (ts : list token) (k : stack) : option (list cointro_pat) :=
+  match ts with
+  | [] => close k []
+  | TParenL :: ts => parse_go ts (StList :: k)
+  | TParenR :: ts => k ← close_ident k []; parse_go ts k
+  | TName s :: ts => parse_go ts (StPat (SCoHyp s) :: k)
+  | TPure x :: ts => parse_go ts (StPat (SPureGoal false) :: k)
+  | TBracketL :: TPure None :: TBracketR :: ts =>
+     parse_go ts (StPat (SPureGoal false) :: k)
+  | TBracketL :: TPure None :: TDone :: TBracketR :: ts =>
+     parse_go ts (StPat (SPureGoal true) :: k)
+  | TBracketL :: TIntuitionistic :: ts => parse_goal ts GIntuitionistic false [] k
+  | TBracketL :: TModal :: ts => parse_goal ts GModal false [] k
+  | TBracketL :: ts => parse_goal ts GSpatial false [] k
+  | _ => None
+  end
+with parse_goal (ts : list token)
+    (ki : goal_kind) (neg : bool) (hyps : list ident)
+    (k : stack) : option (list cointro_pat) :=
+  match ts with
+  | TName s :: ts => parse_goal ts ki neg (INamed s :: hyps) k
+  | TMinus :: ts =>
+     guard (¬neg ∧ hyps = []); parse_goal ts ki true hyps k
+  | TBracketR :: ts =>
+     parse_go ts (StPat (SSplitGoal (SpecGoal ki neg (reverse hyps))) :: k)
+  | _ => None
+  end.
+Definition parse (s : string) : option (list cointro_pat) :=
+  parse_go (tokenize s) [].
+
+Ltac parse s :=
+  lazymatch type of s with
+  | list cointro_pat => s
+  | cointro_pat => constr:([s])
+  | string =>
+     lazymatch eval vm_compute in (parse s) with
+     | Some ?pats => pats
+     | _ => fail "cointro_pat.parse: cannot parse" s "as a cointroduction pattern"
+     end
+  | ident => constr:([SCoHyp s])
+  | ?X => fail "cointro_pat.parse: the term" s
+     "is expected to be a cointroduction pattern"
+     "(usually a string),"
+     "but has unexpected type" X
+  end.
+End cointro_pat.
